Use PMap for ctrl plane variables, update proofs.

CrProgramState.v
@@ -1,11 +1,12 @@
 From MyProject Require Export CrIdentifiers.
+From MyProject Require Export Maps.
 Require Import Strings.String.
 Require Import ZArith.
 
 (* Current values for each of these identifiers as a map *)
 Definition HeaderMap (T : Type) := Header -> T.
 Definition StateVarMap (T : Type) := StateVar -> T.
-Definition CtrlPlaneConfigNameMap (T : Type) := CtrlPlaneConfigName -> T.
+Definition CtrlPlaneConfigNameMap (T : Type) := PMap.t T.
 
 (* The ProgramState is a record containing three maps:,
    one each for mapping headers/statevars/ctrlplaneconfigs to their current values *)
@@ -17,7 +18,7 @@ Record ProgramState (T : Type) := {
 
 Arguments header_map {T} _ _.
 Arguments state_var_map {T} _ _.  
-Arguments ctrl_plane_map {T} _ _.
+Arguments ctrl_plane_map {T} _.
 
 Definition lookup_hdr {T : Type} (s: ProgramState T) (x: Header) : T :=
   header_map s x.
@@ -28,11 +29,11 @@ Definition lookup_state {T : Type} (s: ProgramState T) (x: StateVar) : T :=
 Opaque lookup_state.
 
 Definition lookup_ctrl {T : Type} (s: ProgramState T) (x: CtrlPlaneConfigName) : T :=
-  ctrl_plane_map s x.
+  PMap.get (match x with | CtrlPlaneConfigNameCtr id => id end) (ctrl_plane_map s).
 Opaque lookup_ctrl.
 
 Definition program_state_mapper {T1 T2 : Type} (fc: T1 -> T2) (fh : T1 -> T2) (fs : T1 -> T2) (s: ProgramState T1) : ProgramState T2 :=
-  {| ctrl_plane_map := fun x => fc (lookup_ctrl s x);
+  {| ctrl_plane_map := PMap.map fc (ctrl_plane_map s);
      header_map := fun x => fh (lookup_hdr s x);
      state_var_map := fun x => fs (lookup_state s x) |}.
 Opaque program_state_mapper.
@@ -41,13 +42,11 @@ Definition update_all_hdrs {T : Type} (s: ProgramState T) (fh: Header -> T) : Pr
   {| ctrl_plane_map := ctrl_plane_map s;
      header_map := fun h => fh h;
      state_var_map := state_var_map s |}.
-Opaque update_all_hdrs.
 
 Definition update_all_states {T : Type} (s: ProgramState T) (fs: StateVar -> T) : ProgramState T :=
   {| ctrl_plane_map := ctrl_plane_map s;
      header_map := header_map s;
      state_var_map := fun sv => fs sv |}.
-Opaque update_all_states.
 
 Definition update_hdr {T : Type} (s: ProgramState T) (x: Header) (v: T) : ProgramState T :=
   {| ctrl_plane_map := ctrl_plane_map s;
@@ -55,7 +54,6 @@ Definition update_hdr {T : Type} (s: ProgramState T) (x: Header) (v: T) : Progra
             | HeaderCtr x_id, HeaderCtr y_id => if Pos.eqb x_id y_id then v else lookup_hdr s y
            end;
      state_var_map := state_var_map s|}.
-Opaque update_hdr.
 
 Definition update_state {T : Type} (s: ProgramState T) (x: StateVar) (v: T) : ProgramState T :=
   {| ctrl_plane_map := ctrl_plane_map s;
@@ -64,3 +62,38 @@ Definition update_state {T : Type} (s: ProgramState T) (x: StateVar) (v: T) : Pr
             | StateVarCtr x_id, StateVarCtr y_id => if Pos.eqb x_id y_id then v else lookup_state s y
            end |}.
 Opaque update_state.
+
+Lemma ctrl_plane_invariant_update_hdr:
+  forall {T} (s: ProgramState T) (x: Header) (v: T),
+    ctrl_plane_map (update_hdr s x v) = ctrl_plane_map s.
+Proof.
+  intros.
+  unfold update_hdr.
+  destruct x; simpl; try reflexivity.
+Qed.
+
+Lemma ctrl_plane_invariant_update_hdrs:
+  forall {T} (s: ProgramState T) (f: Header -> T),
+    ctrl_plane_map (update_all_hdrs s f) = ctrl_plane_map s.
+Proof.
+  intros.
+  unfold update_all_hdrs.
+  simpl.
+  reflexivity.
+Qed.
+
+(* Same as above but for state vars *)
+
+Lemma ctrl_plane_invariant_update_states:
+  forall {T} (s: ProgramState T) (f: StateVar -> T),
+    ctrl_plane_map (update_all_states s f) = ctrl_plane_map s.
+Proof.
+  intros.
+  unfold update_all_states.
+  simpl.
+  reflexivity.
+Qed.
+
+Opaque update_hdr.
+Opaque update_all_hdrs.
+Opaque update_all_states.
