CtrlPlaneInvariantsSmt.v
@@ -1,0 +1,94 @@
+(* Various helper lemmas showing ctrl plane maps don't change *)
+From MyProject Require Import CrTransformer.
+From MyProject Require Import CrIdentifiers.
+From MyProject Require Import CrConcreteSemanticsTransformer.
+From MyProject Require Import SmtExpr.
+From MyProject Require Import CrSymbolicSemanticsTransformer.
+Require Import Coq.Lists.List.
+
+(* Effectively, ctrl plane doesn't change *)
+Lemma ctrl_plane_invariant_hdr_op_smt:
+  forall ho c1,
+  ctrl_plane_map (eval_hdr_op_assign_smt ho c1) =
+  ctrl_plane_map c1.
+Proof.
+  intros ho c1.
+  destruct ho; simpl; try reflexivity.
+Qed.
+
+(* Effectively, ctrl plane doesn't change *)
+Lemma ctrl_plane_invariant_hdr_op_list_smt:
+  forall hol c1,
+  ctrl_plane_map (eval_hdr_op_list_smt hol c1) =
+  ctrl_plane_map c1.
+Proof.
+  intros.
+  induction hol.
+  - reflexivity.
+  - simpl. rewrite <- IHhol.
+    apply ctrl_plane_invariant_hdr_op_smt.
+Qed.
+
+
+Lemma ctrl_plane_invariant_seq_rule_smt:
+  forall s c,
+    ctrl_plane_map (eval_seq_rule_smt s c) =
+    ctrl_plane_map c.
+Proof.
+  intros.
+  unfold eval_seq_rule_smt.
+  destruct s.
+  destruct (eval_match_smt match_pattern c);
+  rewrite ctrl_plane_invariant_update_states;
+  rewrite ctrl_plane_invariant_update_hdrs;
+  reflexivity.
+Qed.
+
+Lemma ctrl_plane_invariant_par_rule_smt:
+  forall p c,
+    ctrl_plane_map (eval_par_rule_smt p c) =
+    ctrl_plane_map c.
+Proof.
+  intros.
+  unfold eval_par_rule_smt.
+  destruct p.
+  destruct (eval_match_smt match_pattern c);
+  rewrite ctrl_plane_invariant_update_states;
+  rewrite ctrl_plane_invariant_update_hdrs;
+  reflexivity.
+Qed.
+
+Lemma ctrl_plane_invariant_ma_rule_smt:
+  forall m c,
+    ctrl_plane_map (eval_match_action_rule_smt m c) =
+    ctrl_plane_map c.
+Proof.
+  intros.
+  unfold eval_match_action_rule_smt.
+  destruct m.
+  - apply ctrl_plane_invariant_seq_rule_smt.
+  - apply ctrl_plane_invariant_par_rule_smt.
+Qed.
+
+Lemma ctrl_plane_invariant_transformer_intermediate_smt:
+  forall a t c,
+    ctrl_plane_map (eval_transformer_smt (a :: t) c) =
+    ctrl_plane_map (eval_transformer_smt t c).
+Proof.
+  intros.
+  unfold eval_transformer_smt.
+  remember (a :: t) as full_list.
+  repeat rewrite ctrl_plane_invariant_update_states.
+  repeat rewrite ctrl_plane_invariant_update_hdrs.
+  reflexivity.
+Qed.
+
+Lemma ctrl_plane_invariant_transformer_smt:
+  forall c t,
+    ctrl_plane_map (eval_transformer_smt t c) = ctrl_plane_map c.
+Proof.
+  intros.
+  induction t.
+  - reflexivity.
+  - rewrite <- IHt. apply ctrl_plane_invariant_transformer_intermediate_smt.
+Qed.
